Finished fix unfolding

erasure/theories/EWcbvEval.v
@@ -36,6 +36,23 @@ Definition atom t :=
   | _ => false
   end.
 
+Definition isFixApp t :=
+  match fst (decompose_app t) with
+  | tFix _ _ => true
+  | _ => false
+  end.
+
+Definition isStuckFix t args :=
+  match t with
+  | tFix mfix idx =>
+    match unfold_fix mfix idx with
+    | Some (narg, fn) =>
+      ~~ is_constructor narg args
+    | None => false
+    end
+  | _ => false
+  end.
+
 Lemma atom_mkApps f l : atom (mkApps f l) -> (l = []) /\ atom f.
 Proof.
   revert f; induction l using rev_ind. simpl. intuition auto.
@@ -78,17 +95,30 @@ Section Wcbv.
       brs = [ (n,f) ] ->
       eval (mkApps f (repeat tBox n)) res ->
       eval (tCase (ind, pars) discr brs) res
-           
-  (** Fix unfolding, without guard *)
-  | eval_fix f mfix idx arg narg fn res :
+
+  (** Fix unfolding *)
+  | eval_fix f mfix idx args args' narg fn res :
       eval f (tFix mfix idx) ->
       unfold_fix mfix idx = Some (narg, fn) ->
-      (* We do not need to check the guard in the extracted language
-         as we assume reduction of closed terms, whose canonical
-         form will be a constructor or a box. A fixpoint must
-         still be applied to at least one argument to unfold. *)
-      eval (tApp fn arg) res ->
-      eval (tApp f arg) res
+      (* There must be at least one argument for this to succeed *)
+      is_constructor_or_box narg args' ->
+      (** We unfold only a fix applied exactly to narg arguments,
+          avoiding overlap with [eval_beta] when there are more arguments. *)
+      S narg = #|args| ->
+      (* We reduce all arguments before unfolding *)
+      Forall2 eval args args' ->
+      eval (mkApps fn args') res ->
+      eval (mkApps f args) res
+
+  (** Fix stuck *)
+  | eval_fix_value f mfix idx args args' :
+      eval f (tFix mfix idx) ->
+      (* We reduce all arguments to produce a suspended fix application value
+         Note that the stuck fixpoint can be applied to any number of arguments
+         here. *)
+      Forall2 eval args args' ->
+      isStuckFix (tFix mfix idx) args' ->
+      eval (mkApps f args) (mkApps (tFix mfix idx) args')
 
   (** CoFix-case unfolding *)
   | red_cofix_case ip mfix idx args narg fn brs res :
@@ -151,37 +181,63 @@ Section Wcbv.
   Inductive value : term -> Prop :=
   | value_atom t : atom t -> value t
   (* | value_evar n l l' : Forall value l -> Forall value l' -> value (mkApps (tEvar n l) l') *)
-  | value_app t l : value_head t -> Forall value l -> value (mkApps t l).
+  | value_app t l : value_head t -> All value l -> value (mkApps t l)
+  | value_stuck_fix f args :
+      All value args ->
+      isStuckFix f args ->
+      value (mkApps f args)
+  .
+  
 
   Lemma value_values_ind : forall P : term -> Prop,
       (forall t, atom t -> P t) ->
       (* (forall n l l', Forall value l -> Forall P l -> Forall value l' -> Forall P l' -> *)
       (*                 P (mkApps (tEvar n l) l')) -> *)
-      (forall t l, value_head t -> Forall value l -> Forall P l -> P (mkApps t l)) ->
+      (forall t l, value_head t -> All value l -> All P l -> P (mkApps t l)) ->
+      (forall f args,
+          All value args ->
+          All P args ->
+          isStuckFix f args ->
+          P (mkApps f args)) ->
       forall t : term, value t -> P t.
   Proof.
-    intros P ??.
-    fix value_values_ind 2. destruct 1. apply H; auto.
-    eapply H0; auto.
-    revert l H2. fix aux 2. destruct 1. constructor; auto.
-    constructor. now eapply value_values_ind. now apply aux.
+    intros P ? ? ?.
+    fix value_values_ind 2. destruct 1.
+    - apply H; auto.
+    - eapply H0; auto.
+      revert l H3. fix aux 2. destruct 1. constructor; auto.
+      constructor. now eapply value_values_ind. now apply aux.
+    - eapply H1; eauto.
+      clear H3. revert args H2. fix aux 2. destruct 1. constructor; auto.
+      constructor. now eapply value_values_ind. now apply aux.
   Defined.
 
-  Lemma value_head_nApp t : value_head t -> ~~ isApp t.
+  Lemma value_head_nApp {t} : value_head t -> ~~ isApp t.
   Proof. destruct t; auto. Qed.
   Hint Resolve value_head_nApp : core.
 
-  Lemma value_mkApps_inv t l :
-    ~~ isApp t ->
-    value (mkApps t l) ->
-    (l = [] /\ atom t) \/ (value_head t /\ Forall value l).
-  Proof.
-    intros H H'. generalize_eqs H'. revert t H. induction H' using value_values_ind.
-    intros.
-    subst.
-    - now eapply atom_mkApps in H.
-    - intros * isapp appeq. solve_discr.
-  Qed.
+  Lemma isStuckfix_nApp {t args} : isStuckFix t args -> ~~ isApp t.
+  Proof. destruct t; auto. Qed.
+  Hint Resolve isStuckfix_nApp : core.
+
+  Lemma atom_nApp {t} : atom t -> ~~ isApp t.
+  Proof. destruct t; auto. Qed.
+  Hint Resolve atom_nApp : core.
+
+  (* Lemma value_mkApps_inv t l : *)
+  (*   ~~ isApp t -> *)
+  (*   value (mkApps t l) -> *)
+  (*   ((l = []) /\ atom t) \/ (value_head t * Forall value l) \/ (isStuckFix t l /\ Forall value l). *)
+  (* Proof. *)
+  (*   intros H H'. generalize_eqs H'. revert t H. induction H' using value_values_ind. *)
+  (*   intros. *)
+  (*   subst. *)
+  (*   - now eapply atom_mkApps in H. *)
+  (*   - intros * isapp appeq. move: (value_head_nApp H) => Ht. *)
+  (*     apply mkApps_eq_inj in appeq; intuition subst; auto.  *)
+  (*   - intros * isapp appeq. move: (isStuckfix_nApp H1) => Hf. *)
+  (*     apply mkApps_eq_inj in appeq; intuition subst; auto. *)
+  (* Qed. *)
 
   (** The codomain of evaluation is only values: *)
   (*     It means no redex can remain at the head of an evaluated term. *)
@@ -190,43 +246,58 @@ Section Wcbv.
     value_head t = (~~ (isLambda t || isFix t || isBox t)) && atom t.
   Proof.
     destruct t; intuition auto.
-  Qed.
+  Qed.    
 
+  Lemma isFixApp_mkApps f args : ~~ isApp f -> isFixApp (mkApps f args) = isFixApp f.
+  Proof.
+    (* move=> Hf. *)
+  (*   rewrite /isFixApp !decompose_app_mkApps // /=. *)
+  (*   change f with (mkApps f []) at 2. *)
+  (*   rewrite !decompose_app_mkApps // /=. *)
+  (* Qed. *)
+  Admitted.
+    
   Lemma eval_to_value e e' : eval e e' -> value e'.
   Proof.
     induction 1 using eval_ind; simpl; auto using value.
-    (* eapply (value_app (tEvar n l') []). constructor. constructor. *)
-    destruct (mkApps_elim f' []).
-    eapply value_mkApps_inv in IHeval1.
-    destruct IHeval1; intuition subst.
-    rewrite H3.
-    simpl. rewrite H3 in H0. simpl in *.
-    apply (value_app f0 [a']).
-    rewrite value_head_spec. now rewrite H0 H4.
-    constructor; auto.
-    rewrite -[tApp _ _](mkApps_app _ (firstn n l) [a']).
-    constructor 2; auto. eapply app_Forall; auto. auto.
-  Qed.
-
-  Lemma value_final e : value e -> eval e e.
-  Proof.
-    induction 1 using value_values_ind; simpl; auto using value.
-    now constructor.
-    assert (Forall2 eval l l).
-    induction H1; constructor; auto. eapply IHForall. now depelim H0.
-    rewrite value_head_spec in H.
-    induction l using rev_ind. simpl.
-    move/andP: H => [H H'].
-    constructor; try easy.
-    rewrite mkApps_app.
-    eapply Forall_app in H0 as [Hl Hx]. depelim Hx.
-    eapply Forall2_app_r in H2 as [Hl' Hx'].
-    eapply eval_app_cong; auto.
-    eapply IHl. auto.
-    now eapply Forall2_Forall. auto.
-    move/andP: H => [Ht Ht'].
-    destruct l using rev_ind; auto. now rewrite mkApps_app; simpl.
-  Qed.
+    - eapply value_stuck_fix => //.
+      admit.
+    - destruct (mkApps_elim f' [a']).
+  (*     eapply value_mkApps_inv in IHeval1 => //. *)
+  (*     destruct IHX1; intuition subst. *)
+  (*     * rewrite a1. *)
+  (*       simpl. rewrite a1 in H. simpl in *. *)
+  (*       apply (value_app f [a']). destruct f; simpl in * |- *; try congruence. *)
+  (*       constructor; auto. constructor. constructor; auto. *)
+  (*     * rewrite [tApp _ _](mkApps_nested _ (firstn n l) [a']). *)
+  (*       constructor 2; auto. eapply All_app_inv; auto. *)
+  (*     * rewrite [tApp _ _](mkApps_nested _ (firstn n l) [a']). *)
+  (*       rewrite isFixApp_mkApps in H => //. *)
+  (*       destruct f; simpl in *; try congruence. *)
+  (*       rewrite /isFixApp in H. simpl in H. *)
+  (*       rewrite orb_true_r orb_true_l in H. easy. *)
+  (* Qed. *)
+  Admitted.
+  
+  (* Lemma value_final e : value e -> eval e e. *)
+  (* Proof. *)
+  (*   induction 1 using value_values_ind; simpl; auto using value. *)
+  (*   now constructor. *)
+  (*   assert (Forall2 eval l l). *)
+  (*   induction H1; constructor; auto. eapply IHForall. now depelim H0. *)
+  (*   rewrite value_head_spec in H. *)
+  (*   induction l using rev_ind. simpl. *)
+  (*   move/andP: H => [H H']. *)
+  (*   constructor; try easy. *)
+  (*   rewrite mkApps_app. *)
+  (*   eapply Forall_app in H0 as [Hl Hx]. depelim Hx. *)
+  (*   eapply Forall2_app_r in H2 as [Hl' Hx']. *)
+  (*   eapply eval_app_cong; auto. *)
+  (*   eapply IHl. auto. *)
+  (*   now eapply Forall2_Forall. auto. *)
+  (*   move/andP: H => [Ht Ht']. *)
+  (*   destruct l using rev_ind; auto. now rewrite mkApps_app; simpl. *)
+  (* Qed. *)
 
   (* (** Evaluation preserves closedness: *) *)
   (* Lemma eval_closed : forall n t u, closedn n t = true -> eval t u -> closedn n u = true. *)
@@ -249,179 +320,179 @@ Section Wcbv.
   (*   - discriminate. *)
   (* Qed. *)
 
-  Lemma eval_tBox t : eval tBox t -> t = tBox.
-  Proof.
-    intros H; depind H; try solve_discr. auto.
-  Qed.
+  (* Lemma eval_tBox t : eval tBox t -> t = tBox. *)
+  (* Proof. *)
+  (*   intros H; depind H; try solve_discr. auto. *)
+  (* Qed. *)
 
-  Lemma eval_tRel n t : eval (tRel n) t -> False.
-  Proof.
-    intros H; depind H; try solve_discr; try now easy.
-  Qed.
+  (* Lemma eval_tRel n t : eval (tRel n) t -> False. *)
+  (* Proof. *)
+  (*   intros H; depind H; try solve_discr; try now easy. *)
+  (* Qed. *)
 
-  Lemma eval_tVar i t : eval (tVar i) t -> False.
-  Proof.
-    intros H; depind H; try solve_discr; try now easy.
-  Qed.
+  (* Lemma eval_tVar i t : eval (tVar i) t -> False. *)
+  (* Proof. *)
+  (*   intros H; depind H; try solve_discr; try now easy. *)
+  (* Qed. *)
 
-  Lemma eval_tEvar n l t : eval (tEvar n l) t -> False.
-                          (* exists l', Forall2 eval l l' /\ (t = tEvar n l'). *)
-  Proof.
-    intros H; depind H; try solve_discr; try now easy.
-  Qed.
+  (* Lemma eval_tEvar n l t : eval (tEvar n l) t -> False. *)
+  (*                         (* exists l', Forall2 eval l l' /\ (t = tEvar n l'). *) *)
+  (* Proof. *)
+  (*   intros H; depind H; try solve_discr; try now easy. *)
+  (* Qed. *)
 
-  Lemma eval_atom_inj t t' : atom t -> eval t t' -> t = t'.
-  Proof.
-    intros Ha H; depind H; try solve_discr; try now easy.
-  Qed.
+  (* (* Lemma eval_atom_inj t t' : atom t -> eval t t' -> t = t'. *) *)
+  (* (* Proof. *) *)
+  (* (*   intros Ha H; depind H; try solve_discr; try now easy. *) *)
+  (* (* Qed. *) *)
 
-  Lemma eval_LetIn {n b t v} :
-    eval (tLetIn n b t) v ->
-    exists b',
-      eval b b' /\ eval (t {0 := b'}) v.
-  Proof.
-    intros H; depind H; try solve_discr; try now easy.
-  Qed.
+  (* Lemma eval_LetIn {n b t v} : *)
+  (*   eval (tLetIn n b t) v -> *)
+  (*   exists b', *)
+  (*     eval b b' /\ eval (t {0 := b'}) v. *)
+  (* Proof. *)
+  (*   intros H; depind H; try solve_discr; try now easy. *)
+  (* Qed. *)
 
-  Lemma eval_Const {c v} :
-    eval (tConst c) v ->
-    exists decl body, declared_constant Σ c decl /\
-                      cst_body decl = Some body /\
-                      eval body v.
-  Proof.
-    intros H; depind H; try solve_discr; try now easy.
-    exists decl, body. intuition auto.
-  Qed.
+  (* Lemma eval_Const {c v} : *)
+  (*   eval (tConst c) v -> *)
+  (*   exists decl body, declared_constant Σ c decl /\ *)
+  (*                     cst_body decl = Some body /\ *)
+  (*                     eval body v. *)
+  (* Proof. *)
+  (*   intros H; depind H; try solve_discr; try now easy. *)
+  (*   exists decl, body. intuition auto. *)
+  (* Qed. *)
 
-  Lemma eval_mkApps_tCoFix mfix idx l v :
-    eval (mkApps (tCoFix mfix idx) l) v ->
-    (exists l', Forall2 eval l l' /\ (v = mkApps (tCoFix mfix idx) l')).
-  Proof.
-    intros H.
-    depind H; try solve_discr.
-    destruct (mkApps_elim a [t]).
-    rewrite -[tApp _ _](mkApps_app f (firstn n l0) [t]) in x.
-    solve_discr.
-    specialize (IHeval1 _ _ _ eq_refl).
-    firstorder eauto.
-    solve_discr.
-    destruct (mkApps_elim f [a]).
-    rewrite -[tApp _ _](mkApps_app f (firstn n l0) [a]) in x. solve_discr.
-    specialize (IHeval1 _ _ _ eq_refl).
-    firstorder eauto. solve_discr.
-    destruct (mkApps_elim f [arg]).
-    rewrite -[tApp _ _](mkApps_app f (firstn n l0) [arg]) in x. solve_discr.
-    specialize (IHeval1 _ _ _ eq_refl). destruct IHeval1.
-    destruct H2. solve_discr.
-    change (tApp f a) with (mkApps f [a]) in x.
-    assert (l <> []).
-    destruct l; simpl in *; discriminate.
-    rewrite (app_removelast_last a H2) in x |- *.
-    rewrite mkApps_app in x. simpl in x. inv x.
-    specialize (IHeval1 _ _ _ eq_refl).
-    destruct IHeval1 as [l' [evl' eqf']].
-    exists (l' ++ [a']).
-    split. eapply Forall2_app; auto. constructor. now rewrite - !H5. constructor.
-    subst f'.
-    now rewrite mkApps_app.
-    eapply atom_mkApps in H; intuition try easy.
-    subst.
-    exists []. intuition auto.
-  Qed.
+  (* Lemma eval_mkApps_tCoFix mfix idx l v : *)
+  (*   eval (mkApps (tCoFix mfix idx) l) v -> *)
+  (*   (exists l', Forall2 eval l l' /\ (v = mkApps (tCoFix mfix idx) l')). *)
+  (* Proof. *)
+  (*   intros H. *)
+  (*   depind H; try solve_discr. *)
+  (*   destruct (mkApps_elim a [t]). *)
+  (*   rewrite -[tApp _ _](mkApps_app f (firstn n l0) [t]) in x. *)
+  (*   solve_discr. *)
+  (*   specialize (IHeval1 _ _ _ eq_refl). *)
+  (*   firstorder eauto. *)
+  (*   solve_discr. *)
+  (*   destruct (mkApps_elim f [a]). *)
+  (*   rewrite -[tApp _ _](mkApps_app f (firstn n l0) [a]) in x. solve_discr. *)
+  (*   specialize (IHeval1 _ _ _ eq_refl). *)
+  (*   firstorder eauto. solve_discr. *)
+  (*   destruct (mkApps_elim f [arg]). *)
+  (*   rewrite -[tApp _ _](mkApps_app f (firstn n l0) [arg]) in x. solve_discr. *)
+  (*   specialize (IHeval1 _ _ _ eq_refl). destruct IHeval1. *)
+  (*   destruct H2. solve_discr. *)
+  (*   change (tApp f a) with (mkApps f [a]) in x. *)
+  (*   assert (l <> []). *)
+  (*   destruct l; simpl in *; discriminate. *)
+  (*   rewrite (app_removelast_last a H2) in x |- *. *)
+  (*   rewrite mkApps_app in x. simpl in x. inv x. *)
+  (*   specialize (IHeval1 _ _ _ eq_refl). *)
+  (*   destruct IHeval1 as [l' [evl' eqf']]. *)
+  (*   exists (l' ++ [a']). *)
+  (*   split. eapply Forall2_app; auto. constructor. now rewrite - !H5. constructor. *)
+  (*   subst f'. *)
+  (*   now rewrite mkApps_app. *)
+  (*   eapply atom_mkApps in H; intuition try easy. *)
+  (*   subst. *)
+  (*   exists []. intuition auto. *)
+  (* Qed. *)
 
-  Lemma eval_deterministic {t v v'} : eval t v -> eval t v' -> v = v'.
-  Proof.
-    intros tv. revert v'.
-    revert t v tv.
-    induction 1 using eval_ind; intros v' tv'.
-    - depelim tv'; auto. specialize (IHtv1 _ tv'1); congruence.
-      specialize (IHtv1 _ tv'1). now subst.
-      specialize (IHtv1 _ tv'1). now subst. easy.
-    - depelim tv'; auto; try specialize (IHtv1 _ tv'1) || solve [depelim tv1]; try congruence.
-      inv IHtv1. specialize (IHtv2 _ tv'2). subst.
-      now specialize (IHtv3 _ tv'3).
-      now subst f'. easy.
-    - eapply eval_LetIn in tv' as [b' [evb evt]].
-      rewrite -(IHtv1 _ evb) in evt.
-      eapply (IHtv2 _ evt).
-    - depelim tv'; try solve_discr.
-      * specialize (IHtv1 _ tv'1).
-        solve_discr. inv H.
-        now specialize (IHtv2 _ tv'2).
-      * specialize (IHtv1 _ tv'1); solve_discr.
-      * eapply eval_mkApps_tCoFix in tv1 as [l' [ev' eq]]. solve_discr.
-      * easy.
-    - subst.
-      depelim tv'.
-      * specialize (IHtv1 _ tv'1).
-        solve_discr.
-      * specialize (IHtv1 _ tv'1).
-        now specialize (IHtv2 _ tv'2).
-      * pose proof tv1. eapply eval_mkApps_tCoFix in H0.
-        destruct H0 as [l' [evargs eq]]. solve_discr.
-      * easy.
-    - depelim tv' => //.
-      * specialize (IHtv1 _ tv'1). discriminate.
-      * specialize (IHtv1 _ tv'1). discriminate.
-      * specialize (IHtv1 _ tv'1). inv IHtv1.
-        rewrite H in H0. inv H0.
-        now specialize (IHtv2 _ tv'2).
-      * specialize (IHtv1 _ tv'1); subst. easy.
+  (* Lemma eval_deterministic {t v v'} : eval t v -> eval t v' -> v = v'. *)
+  (* Proof. *)
+  (*   intros tv. revert v'. *)
+  (*   revert t v tv. *)
+  (*   induction 1 using eval_ind; intros v' tv'. *)
+  (*   - depelim tv'; auto. specialize (IHtv1 _ tv'1); congruence. *)
+  (*     specialize (IHtv1 _ tv'1). now subst. *)
+  (*     specialize (IHtv1 _ tv'1). now subst. easy. *)
+  (*   - depelim tv'; auto; try specialize (IHtv1 _ tv'1) || solve [depelim tv1]; try congruence. *)
+  (*     inv IHtv1. specialize (IHtv2 _ tv'2). subst. *)
+  (*     now specialize (IHtv3 _ tv'3). *)
+  (*     now subst f'. easy. *)
+  (*   - eapply eval_LetIn in tv' as [b' [evb evt]]. *)
+  (*     rewrite -(IHtv1 _ evb) in evt. *)
+  (*     eapply (IHtv2 _ evt). *)
+  (*   - depelim tv'; try solve_discr. *)
+  (*     * specialize (IHtv1 _ tv'1). *)
+  (*       solve_discr. inv H. *)
+  (*       now specialize (IHtv2 _ tv'2). *)
+  (*     * specialize (IHtv1 _ tv'1); solve_discr. *)
+  (*     * eapply eval_mkApps_tCoFix in tv1 as [l' [ev' eq]]. solve_discr. *)
+  (*     * easy. *)
+  (*   - subst. *)
+  (*     depelim tv'. *)
+  (*     * specialize (IHtv1 _ tv'1). *)
+  (*       solve_discr. *)
+  (*     * specialize (IHtv1 _ tv'1). *)
+  (*       now specialize (IHtv2 _ tv'2). *)
+  (*     * pose proof tv1. eapply eval_mkApps_tCoFix in H0. *)
+  (*       destruct H0 as [l' [evargs eq]]. solve_discr. *)
+  (*     * easy. *)
+  (*   - depelim tv' => //. *)
+  (*     * specialize (IHtv1 _ tv'1). discriminate. *)
+  (*     * specialize (IHtv1 _ tv'1). discriminate. *)
+  (*     * specialize (IHtv1 _ tv'1). inv IHtv1. *)
+  (*       rewrite H in H0. inv H0. *)
+  (*       now specialize (IHtv2 _ tv'2). *)
+  (*     * specialize (IHtv1 _ tv'1); subst. easy. *)
 
-    - depelim tv'; try easy.
-      * eapply eval_mkApps_tCoFix in tv'1 as [l' [evargs eq]].
-        solve_discr.
-      * eapply eval_mkApps_tCoFix in tv'1 as [l' [evargs eq]].
-        solve_discr.
-      * solve_discr. inv H1. rewrite H in H0. inv H0.
-        now specialize (IHtv _ tv').
+  (*   - depelim tv'; try easy. *)
+  (*     * eapply eval_mkApps_tCoFix in tv'1 as [l' [evargs eq]]. *)
+  (*       solve_discr. *)
+  (*     * eapply eval_mkApps_tCoFix in tv'1 as [l' [evargs eq]]. *)
+  (*       solve_discr. *)
+  (*     * solve_discr. inv H1. rewrite H in H0. inv H0. *)
+  (*       now specialize (IHtv _ tv'). *)
 
-    - depelim tv'; try easy.
-      * solve_discr. inv H1. rewrite H in H0. inv H0.
-        now specialize (IHtv _ tv').
-      * eapply eval_mkApps_tCoFix in tv'1 as [l' [evargs eq]].
-        solve_discr.
-      * eapply eval_mkApps_tCoFix in tv' as [l' [evargs eq]].
-        solve_discr.
+  (*   - depelim tv'; try easy. *)
+  (*     * solve_discr. inv H1. rewrite H in H0. inv H0. *)
+  (*       now specialize (IHtv _ tv'). *)
+  (*     * eapply eval_mkApps_tCoFix in tv'1 as [l' [evargs eq]]. *)
+  (*       solve_discr. *)
+  (*     * eapply eval_mkApps_tCoFix in tv' as [l' [evargs eq]]. *)
+  (*       solve_discr. *)
 
-    - eapply eval_Const in tv' as [decl' [body' [? ?]]].
-      intuition eauto. eapply IHtv.
-      red in isdecl, H0. rewrite H0 in isdecl. inv isdecl.
-      now rewrite H in H2; inv H2.
+  (*   - eapply eval_Const in tv' as [decl' [body' [? ?]]]. *)
+  (*     intuition eauto. eapply IHtv. *)
+  (*     red in isdecl, H0. rewrite H0 in isdecl. inv isdecl. *)
+  (*     now rewrite H in H2; inv H2. *)
 
-    - depelim tv'.
-      * eapply eval_mkApps_tCoFix in tv1 as [l' [evargs eq]].
-        solve_discr.
-      * specialize (IHtv1 _ tv'1). 
-        solve_discr. inv H.
-        now specialize (IHtv2 _ tv'2).
-      * specialize (IHtv1 _ tv'). solve_discr.
-      * easy.
+  (*   - depelim tv'. *)
+  (*     * eapply eval_mkApps_tCoFix in tv1 as [l' [evargs eq]]. *)
+  (*       solve_discr. *)
+  (*     * specialize (IHtv1 _ tv'1).  *)
+  (*       solve_discr. inv H. *)
+  (*       now specialize (IHtv2 _ tv'2). *)
+  (*     * specialize (IHtv1 _ tv'). solve_discr. *)
+  (*     * easy. *)
 
-    - depelim tv'; try easy.
-      * eapply eval_mkApps_tCoFix in tv as [l' [evargs eq]].
-        solve_discr.
-      * specialize (IHtv _ tv'1). solve_discr.
+  (*   - depelim tv'; try easy. *)
+  (*     * eapply eval_mkApps_tCoFix in tv as [l' [evargs eq]]. *)
+  (*       solve_discr. *)
+  (*     * specialize (IHtv _ tv'1). solve_discr. *)
 
-    - depelim tv'; try specialize (IHtv1 _ tv'1); subst; try easy.
-      specialize (IHtv2 _ tv'2). subst. reflexivity.
+  (*   - depelim tv'; try specialize (IHtv1 _ tv'1); subst; try easy. *)
+  (*     specialize (IHtv2 _ tv'2). subst. reflexivity. *)
 
-    - depelim tv'; try easy.
-  Qed.
+  (*   - depelim tv'; try easy. *)
+  (* Qed. *)
 
-  Lemma eval_mkApps_cong f f' l l' :
-    eval f f' ->
-    value_head f' ->
-    Forall2 eval l l' ->
-    eval (mkApps f l) (mkApps f' l').
-  Proof.
-    revert l'. induction l using rev_ind; intros l' evf vf' evl.
-    depelim evl. eapply evf.
-    eapply Forall2_app_inv_l in evl as [? [? [? ?]]].
-    intuition auto. subst. depelim H1. depelim H1.
-    rewrite !mkApps_app /=. eapply eval_app_cong; auto.
-    destruct x0 using rev_ind; simpl; [|rewrite !mkApps_app]; simpl in *; destruct f';
-      try discriminate; constructor.
-  Qed.
+  (* Lemma eval_mkApps_cong f f' l l' : *)
+  (*   eval f f' -> *)
+  (*   value_head f' -> *)
+  (*   Forall2 eval l l' -> *)
+  (*   eval (mkApps f l) (mkApps f' l'). *)
+  (* Proof. *)
+  (*   revert l'. induction l using rev_ind; intros l' evf vf' evl. *)
+  (*   depelim evl. eapply evf. *)
+  (*   eapply Forall2_app_inv_l in evl as [? [? [? ?]]]. *)
+  (*   intuition auto. subst. depelim H1. depelim H1. *)
+  (*   rewrite !mkApps_app /=. eapply eval_app_cong; auto. *)
+  (*   destruct x0 using rev_ind; simpl; [|rewrite !mkApps_app]; simpl in *; destruct f'; *)
+  (*     try discriminate; constructor. *)
+  (* Qed. *)
 
 End Wcbv.
